wip: remove UScalar/IScalar from Scalar/Ops

backends/lean/Aeneas/Std/Scalar/Ops/Add.lean
@@ -11,23 +11,12 @@ open Result Error Arith ScalarElab WP
 /-!
 # Addition: Definitions
 -/
-def UScalar.add {ty : UScalarTy} (x y : UScalar ty) : Result (UScalar ty) :=
-  UScalar.tryMk ty (x.toNat + y.toNat)
-
-def IScalar.add {ty : IScalarTy} (x y : IScalar ty) : Result (IScalar ty) :=
-  IScalar.tryMk ty (x.toInt + y.toInt)
 
 uscalar def «%S».add (x y : «%S») : Result «%S» :=
   tryMk (x.toNat + y.toNat)
 
 iscalar def «%S».add (x y : «%S») : Result «%S» :=
   tryMk (x.toInt + y.toInt)
-
-def UScalar.try_add {ty : UScalarTy} (x y : UScalar ty) : Option (UScalar ty) :=
-  Option.ofResult (add x y)
-
-def IScalar.try_add {ty : IScalarTy} (x y : IScalar ty) : Option (IScalar ty) :=
-  Option.ofResult (add x y)
 
 scalar def «%S».try_add (x y : «%S») : Option «%S» :=
   Option.ofResult (add x y)
@@ -37,36 +26,12 @@ class ResultAdd (α : Type u) where
 
 infixl:65 " +? " => ResultAdd.add
 
-instance {ty} : ResultAdd (UScalar ty) where
-  add x y := UScalar.add x y
-
-instance {ty} : ResultAdd (IScalar ty) where
-  add x y := IScalar.add x y
-
 scalar instance : ResultAdd «%S» where
   add x y := «%S».add x y
 
 /-!
 # Addition: Theorems
 -/
-
-theorem UScalar.add_equiv {ty} (x y : UScalar ty) :
-  match x +? y with
-  | ok z => x.toNat + y.toNat < 2^ty.numBits ∧
-    z.toNat = x.toNat + y.toNat ∧
-    z.toBitVec = x.toBitVec + y.toBitVec
-  | fail _ => ¬ (UScalar.inBounds ty (x.toNat + y.toNat))
-  | _ => ⊥ := by
-  have : x +? y = add x y := by rfl
-  rw [this]
-  simp [add]
-  have h := tryMk_eq ty (↑x + ↑y)
-  simp [inBounds] at h
-  split at h <;> simp_all
-  zify; simp
-  zify at h
-  have := @Int.emod_eq_of_lt (x.toNat + y.toNat) (2^ty.numBits) (by omega) (by omega)
-  simp [*]
 
 uscalar theorem «%S».add_equiv (x y : «%S») :
   match x +? y with
@@ -85,25 +50,6 @@ uscalar theorem «%S».add_equiv (x y : «%S») :
   zify at h
   have := @Int.emod_eq_of_lt (x.toNat + y.toNat) «%S».size (by omega) (by scalar_tac)
   simp_all [size_eq]
-
-theorem IScalar.add_equiv {ty} (x y : IScalar ty) :
-  match x +? y with
-  | ok z =>
-    IScalar.inBounds ty (x.toInt + y.toInt) ∧
-    z.toInt = x.toInt + y.toInt ∧
-    z.toBitVec = x.toBitVec + y.toBitVec
-  | fail _ => ¬ (IScalar.inBounds ty (x.toInt + y.toInt))
-  | _ => ⊥ := by
-  have : x +? y = add x y := by rfl
-  rw [this]
-  simp [add]
-  have h := tryMk_eq ty (↑x + ↑y)
-  simp [inBounds] at h
-  split at h <;> simp_all
-  apply BitVec.eq_of_toInt_eq
-  simp
-  have := bmod_pow_numBits_eq_of_lt ty (x.toInt + y.toInt) (by omega) (by omega)
-  simp [*]
 
 iscalar theorem «%S».add_equiv (x y : «%S») :
   match x +? y with
