backends/lean/Aeneas/Std/Scalar/Ops/Div.lean
@@ -12,16 +12,6 @@ open Result Error Arith ScalarElab WP
 # Division: Definitions
 -/
 
-def UScalar.div {ty : UScalarTy} (x y : UScalar ty) : Result (UScalar ty) :=
-  if y.toBitVec != 0 then ok ⟨ BitVec.udiv x.toBitVec y.toBitVec ⟩ else fail divisionByZero
-
-def IScalar.div {ty : IScalarTy} (x y : IScalar ty): Result (IScalar ty) :=
-  if y.toInt != 0 then
-    -- There can be an overflow if `x` is equal to the lower bound and `y` to `-1`
-    if ¬ (x.toInt = IScalar.min ty && y.toInt = -1) then ok ⟨ BitVec.sdiv x.toBitVec y.toBitVec ⟩
-    else fail integerOverflow
-  else fail divisionByZero
-
 uscalar def «%S».div (x y : «%S») : Result «%S» :=
   if y.toBitVec != 0 then ok ⟨ BitVec.udiv x.toBitVec y.toBitVec ⟩ else fail divisionByZero
 
@@ -31,22 +21,10 @@ iscalar def «%S».div (x y : «%S») : Result «%S» :=
     else fail integerOverflow
   else fail divisionByZero
 
-def UScalar.try_div {ty : UScalarTy} (x y : UScalar ty) : Option (UScalar ty) :=
-  Option.ofResult (div x y)
-
-def IScalar.try_div {ty : IScalarTy} (x y : IScalar ty): Option (IScalar ty) :=
-  Option.ofResult (div x y)
-
 class ResultDiv (α : Type u) where
   div : α → α → Result α
 
 infixl:70 " /? " => ResultDiv.div
-
-instance {ty} : ResultDiv (UScalar ty) where
-  div x y := UScalar.div x y
-
-instance {ty} : ResultDiv (IScalar ty) where
-  div x y := IScalar.div x y
 
 scalar instance : ResultDiv «%S» where
   div x y := «%S».div x y
@@ -95,27 +73,6 @@ end Tests
 Theorems with a specification which use integers and bit-vectors
 -/
 
-/-- Generic theorem - shouldn't be used much -/
-theorem UScalar.div_toBitVec_spec {ty} (x : UScalar ty) {y : UScalar ty}
-  (hzero : y.toNat ≠ 0) :
-  ∃ z, x /? y = ok z ∧ (↑z : Nat) = ↑x / ↑y ∧ z.toBitVec = x.toBitVec / y.toBitVec := by
-  have hzero' : y.toBitVec ≠ 0#ty.numBits := by
-    intro h
-    zify at h
-    simp_all
-  conv => congr; ext; lhs; simp [ResultDiv.div]
-  simp [hzero', div]
-  simp only [toNat]
-  simp
-
-theorem Int.bmod_pow2_IScalarTy_numBits_minus_one (ty : IScalarTy) :
-  Int.bmod (2 ^ (ty.numBits - 1)) (2 ^ ty.numBits) = - 2 ^ (ty.numBits - 1) := by
-  rw [Int.bmod]
-  /- Just doing a case disjunction on the number of bits because
-     those proofs are annoying -/
-  cases ty <;> simp
-  have := System.Platform.numBits_eq
-  cases this <;> simp [*]
 
 iscalar theorem Int.bmod_pow2_'S_numBits_minus_one :
   Int.bmod (2 ^ (%BitWidth - 1)) (2 ^ %BitWidth) = - 2 ^ (%BitWidth - 1) := by
@@ -159,264 +116,15 @@ theorem IScalar.neg_imp_neg_toInt_toNat_mod_pow_eq_neg_toInt {ty} (x : IScalar t
   rw [hyValToNatMod]
   omega
 
-/-- Generic theorem - shouldn't be used much -/
-theorem IScalar.div_toBitVec_spec {ty} {x y : IScalar ty}
-  (hzero : y.toInt ≠ 0) (hNoOverflow : ¬ (x.toInt = IScalar.min ty ∧ y.toInt = -1)) :
-  ∃ z, x /? y = ok z ∧ (↑z : Int) = Int.tdiv ↑x ↑y ∧ z.toBitVec = BitVec.sdiv x.toBitVec y.toBitVec := by
-  conv => congr; ext; lhs; simp only [ResultDiv.div]
-  simp only [div, bne_iff_ne, ne_eq, hzero, not_false_eq_true, ↓reduceIte, Int.reduceNeg,
-    Bool.and_eq_true, decide_eq_true_eq, hNoOverflow, ok.injEq, _root_.exists_eq_left', and_true]
-  simp only [toInt]
-  -- TODO: simplify the proof by using BitVec.toInt_srem
-
-  simp only [BitVec.sdiv_eq, BitVec.udiv_eq, BitVec.udiv_def, BitVec.toNat_neg, toBitVec_toInt_eq]
-  have pow2Ineq : (2^(ty.numBits - 1) : Int) < 2^ty.numBits := by
-    have := ty.numBits_nonzero
-    have : (0 : Int) < 2^(ty.numBits - 1) := by simp only [Nat.ofNat_pos, pow_pos]
-    have : ty.numBits = ty.numBits - 1 + 1 := by omega
-    conv => rhs; rw [this]
-    rw [Int.pow_succ']
-    omega
-  have hxBounds := x.hBounds
-  have hyBounds := y.hBounds
-
-  split
-
-  . -- 0 ≤ x.toBitVec.toInt
-    -- 0 ≤ y.toBitVec.toInt
-    rw [BitVec.toInt_ofNat']
-    simp only [Int.natCast_ediv]
-    have hx : x.toBitVec.toNat = x.toBitVec.toInt := by
-      have := @BitVec.toInt_eq_msb_cond _ x.toBitVec
-      simp_all
-    have hy : y.toBitVec.toNat = y.toBitVec.toInt := by
-      have := @BitVec.toInt_eq_msb_cond _ y.toBitVec
-      simp_all
-    simp only [hx, toBitVec_toInt_eq, hy]
-    simp only [toBitVec_toInt_eq] at hx hy
-    have := @Int.tdiv_nonneg x.toInt y.toInt (by omega) (by omega)
-    have : -2 ^ (ty.numBits - 1) ≤ 0 := by
-      simp only [Left.neg_nonpos_iff, Nat.ofNat_nonneg, pow_nonneg]
-    have : (x.toInt).tdiv y.toInt < 2 ^ (ty.numBits - 1) := by
-      rw [Int.tdiv_eq_ediv]; split <;> try omega
-      have := @Int.ediv_le_self x.toInt y.toInt (by omega)
-      omega
-
-    have hEq := bmod_pow_numBits_eq_of_lt ty (Int.tdiv x.toInt y.toInt) (by omega) (by omega)
-    rw [← hEq]
-    have htdiv : Int.tdiv x.toInt y.toInt = x.toInt / y.toInt := by
-      rw [Int.tdiv_eq_ediv]
-      have : 0 ≤ x.toInt := by omega
-      simp only [this, true_or, ↓reduceIte, add_zero]
-    rw [htdiv]
-
-  . -- 0 ≤ x.toBitVec.toInt
-    -- y.toBitVec.toInt < 0
-    rename_i hxIneq hyIneq
-    have hx := @BitVec.toInt_eq_msb_cond _ x.toBitVec
-    simp only [toBitVec_toInt_eq, hxIneq, Bool.false_eq_true, ↓reduceIte] at hx
-    have hy := @BitVec.toInt_eq_msb_cond _ y.toBitVec
-    simp only [toBitVec_toInt_eq, hyIneq, ↓reduceIte, Nat.cast_pow, Nat.cast_ofNat] at hy
-    have hyNeg : y.toInt < 0 := by
-      have := @BitVec.msb_eq_toInt _ y.toBitVec
-      simp_all
-    have : -2 ^ (ty.numBits - 1) ≤ Int.tdiv x.toInt y.toInt := by
-      have : Int.tdiv x.toInt (-y.toInt) ≤ 2^(ty.numBits - 1) := by
-        rw [Int.tdiv_eq_ediv]
-        have := @Int.ediv_le_self x.toInt (-y.toInt) (by omega)
-        simp only [ne_eq, Int.reduceNeg, not_and, Int.ediv_neg, ge_iff_le] at *
-        have := x.hmax
-        omega
-      replace this := Int.neg_le_neg this
-      simp only [Int.tdiv_neg, neg_neg] at this
-      apply this
-    have hyToNat : 2 ^ ty.numBits - y.toBitVec.toNat = (-y.toInt).toNat := by
-      rw [hy]
-      simp only [neg_sub, Int.toNat_sub']
-      norm_cast
-    rw [BitVec.toInt_neg, BitVec.toInt_ofNat']
-    simp only [Int.natCast_ediv, Int.natCast_emod, Nat.cast_pow, Nat.cast_ofNat]
-    rw [hyToNat]
-    have : ((-y.toInt).toNat : Int) % 2^ty.numBits = -(y.toInt : Int) := by
-      apply IScalar.neg_imp_neg_toInt_toNat_mod_pow_eq_neg_toInt
-      simp only [toBitVec_toInt_eq]; omega
-    rw [this]; clear this
-    simp only [Int.ediv_neg, Int.bmod_neg_bmod, neg_neg]
-    rw [← hx]
-    have : (x.toInt / y.toInt).bmod (2^ty.numBits) = x.toInt / y.toInt := by
-      have : -2 ^ (ty.numBits - 1) ≤ x.toInt / ↑y := by
-        apply Int.le_of_neg_le_neg
-        have : - (x.toInt / y.toInt) = x.toInt / -y.toInt := by simp only [Int.ediv_neg]
-        rw [this]; clear this
-        have := @Int.ediv_le_self x.toInt (-y.toInt) (by omega)
-        omega
-      have : x.toInt / ↑y < 2 ^ (ty.numBits - 1) := by
-        have : 0 < 2 ^ (ty.numBits - 1) := by simp only [Nat.ofNat_pos, pow_pos]
-        have : x.toInt / y.toInt ≤ 0 := by apply Int.ediv_nonpos_of_nonneg_of_nonpos <;> omega
-        omega
-      have := bmod_pow_numBits_eq_of_lt ty (x.toInt / y.toInt) (by omega) (by omega)
-      rw [this]
-
-    rw [this]; clear this
-
-    have : x.toInt.tdiv y.toInt = - (x.toInt.tdiv (-y.toInt)) := by simp only [Int.tdiv_neg, neg_neg]
-    rw [this]
-    have : x.toInt.tdiv (-y.toInt) = (x.toInt) / (-y.toInt) := by
-      have := @Int.tdiv_eq_ediv x.toInt (-y.toInt)
-      rw [this]
-      split <;> omega
-    rw [this]; clear this
-    simp only [Int.ediv_neg, neg_neg]
-
-  . -- x.toBitVec.toInt < 0
-    -- 0 ≤ y.toBitVec.toInt
-    rename_i hxIneq hyIneq
-    have hx := @BitVec.toInt_eq_msb_cond _ x.toBitVec
-    simp only [toBitVec_toInt_eq, hxIneq, ↓reduceIte, Nat.cast_pow, Nat.cast_ofNat] at hx
-    have hy := @BitVec.toInt_eq_msb_cond _ y.toBitVec
-    simp only [toBitVec_toInt_eq, hyIneq, Bool.false_eq_true, ↓reduceIte] at hy
-    have hxNeg : x.toInt < 0 := by
-      have := @BitVec.msb_eq_toInt _ x.toBitVec
-      simp_all
-    have hyPos : 0 ≤ y.toInt := by
-      have := @BitVec.msb_eq_toInt _ y.toBitVec
-      simp_all
-    have : -2 ^ (ty.numBits - 1) ≤ x.toInt / y.toInt := by
-      have := @Int.ediv_le_ediv (-2 ^ (ty.numBits - 1)) x.toInt y.toInt (by omega) (by omega)
-      have := @Int.self_le_ediv x.toInt y.toInt (by omega) (by omega)
-      omega
-    have hxToNat : 2 ^ ty.numBits - x.toBitVec.toNat = (-x.toInt).toNat := by
-      rw [hx]
-      simp only [neg_sub, Int.toNat_sub']
-      norm_cast
-    rw [BitVec.toInt_neg, BitVec.toInt_ofNat']
-    simp only [Int.natCast_ediv, Int.natCast_emod, Nat.cast_pow, Nat.cast_ofNat]
-
-    rw [hxToNat]
-    have : ((-x.toInt).toNat : Int) % 2^ty.numBits = -(x.toInt : Int) := by
-      apply IScalar.neg_imp_neg_toInt_toNat_mod_pow_eq_neg_toInt
-      simp only [toBitVec_toInt_eq]; omega
-    rw [this]; clear this
-
-    /- We have to treat separately the degenerate case where `x` touches the upper bound
-       and `y = 1` -/
-    dcases hxDivY : -x.toInt / y.toInt = 2^(ty.numBits - 1)
-    . rw [← hy]
-      rw [hxDivY]
-      have ⟨ hx, hy ⟩ : x.toInt = - 2^(ty.numBits - 1) ∧ y.toInt = 1 := by
-        have := @Int.le_div_eq_bound_imp_eq (-x.toInt) y.toInt (2^(ty.numBits - 1))
-          (by omega) (by omega) (by omega) (by omega)
-        omega
-      simp only [hx, hy, Int.tdiv_one]
-
-      have : Int.bmod (2 ^ (ty.numBits - 1)) (2 ^ ty.numBits) =
-             - 2 ^ (ty.numBits - 1) :=
-        Int.bmod_pow2_IScalarTy_numBits_minus_one ty
-      rw [this]
-      simp only [neg_neg]
-      rw [this]
-    . have : 0 ≤ (-x.toInt) / y.toInt := by
-        apply Int.ediv_nonneg <;> omega
-      have : -x.toInt / y.toInt < 2^(ty.numBits - 1) := by
-        have : -x.toInt ≤ 2^(ty.numBits - 1) := by omega
-        have := @Int.ediv_le_self (-x.toInt) y.toInt (by omega)
-        omega
-      rw [← hy]
-      have : (-x.toInt / y.toInt).bmod (2 ^ ty.numBits) =
-             (-x.toInt / y.toInt) := by
-        apply bmod_pow_numBits_eq_of_lt ty _ (by omega) (by omega)
-      rw [this]; clear this
-      have : (-(-x.toInt / ↑y)).bmod (2 ^ ty.numBits) =
-             (-(-x.toInt / ↑y)) := by
-        apply bmod_pow_numBits_eq_of_lt ty _ (by omega) (by omega)
-      rw [this]; clear this
-      have : (-x.toInt) / y.toInt = (-x.toInt).tdiv y.toInt := by
-        rw [Int.tdiv_eq_ediv]
-        omega
-
-      rw [this]; simp only [Int.neg_tdiv, neg_neg]
-
-  . -- x.toBitVec.toInt < 0
-    -- y.toBitVec.toInt < 0
-    rename_i hxIneq hyIneq
-    have hx := @BitVec.toInt_eq_msb_cond _ x.toBitVec
-    simp only [toBitVec_toInt_eq, hxIneq, ↓reduceIte, Nat.cast_pow, Nat.cast_ofNat] at hx
-    have hy := @BitVec.toInt_eq_msb_cond _ y.toBitVec
-    simp only [toBitVec_toInt_eq, hyIneq, ↓reduceIte, Nat.cast_pow, Nat.cast_ofNat] at hy
-    have hxNeg : x.toInt < 0 := by
-      have := @BitVec.msb_eq_toInt _ x.toBitVec
-      simp_all
-    have hyNeg : y.toInt < 0 := by
-      have := @BitVec.msb_eq_toInt _ y.toBitVec
-      simp_all
-    have hxToNat : 2 ^ ty.numBits - x.toBitVec.toNat = (-x.toInt).toNat := by
-      rw [hx]
-      simp only [neg_sub, Int.toNat_sub']
-      norm_cast
-    have hyToNat : 2 ^ ty.numBits - y.toBitVec.toNat = (-y.toInt).toNat := by
-      rw [hy]
-      simp only [neg_sub, Int.toNat_sub']
-      norm_cast
-    rw [hxToNat, hyToNat]
-
-    have : (-x.toInt).toNat % 2^ty.numBits = (-x.toInt).toNat := by
-      apply Nat.mod_eq_of_lt
-      omega
-    rw [this]
-    have : (-y.toInt).toNat % 2^ty.numBits = (-y.toInt).toNat := by
-      apply Nat.mod_eq_of_lt
-      omega
-    rw [this]
-
-    rw [BitVec.toInt_ofNat']
-
-    /- We have to treat separately the degenerate case where `x` touches the lower bound
-       and `y = -1`, because then `x / y` actually overflows -/
-    have hxyInBouds : (-x.toInt) / (-y.toInt) ≠ 2^(ty.numBits - 1) := by
-      -- We do the proof by contradiction
-      intro hEq
-      have hContra : x.toInt = - 2^(ty.numBits - 1) ∧ y.toInt = -1 := by
-        have := @Int.le_div_eq_bound_imp_eq (-x.toInt) (-y.toInt) (2^(ty.numBits - 1))
-          (by omega) (by omega) (by omega) (by omega)
-        omega
-      simp only [hContra, min, Int.reduceNeg, and_self, not_true_eq_false] at hNoOverflow
-
-    have : -(2 ^ (ty.numBits - 1) : Int) ≤ ↑((-x.toInt).toNat / (-y.toInt).toNat) := by
-      have := @Int.ediv_nonneg (-x.toInt).toNat (-y.toInt).toNat (by omega) (by omega)
-      have : -(2 ^ (ty.numBits - 1) : Int) ≤ 0 := by
-        simp only [Left.neg_nonpos_iff, Nat.ofNat_nonneg, pow_nonneg]
-      omega
-
-    have : ((-x.toInt).toNat / (-y.toInt).toNat) < (2 ^ (ty.numBits - 1) : Int) := by
-      -- First prove a ≤ bound
-      have hIneq : ((-x.toInt).toNat / (-y.toInt).toNat) ≤ (2 ^ (ty.numBits - 1) : Int) := by
-        have := @Int.ediv_le_self (-x.toInt).toNat (-y.toInt).toNat (by omega)
-        omega
-      -- Then use the hypothesis about the fact that we're not equal to the bound
-      zify at hIneq
-      have : (-x.toInt).toNat = -x.toInt := by omega
-      rw [this] at hIneq; rw [this]
-      have : (-y.toInt).toNat = -y.toInt := by omega
-      rw [this] at hIneq; rw [this]
-      omega
-    have := bmod_pow_numBits_eq_of_lt ty ((-x.toInt).toNat / (-y.toInt).toNat : Nat) (by omega) (by omega)
-    rw [this]
-
-    zify; simp only [Int.ofNat_toNat]
-
-    have : (-x.toInt) ⊔ 0 = -x.toInt := by omega
-    simp only [this]; clear this
-    have : -↑y ⊔ 0 = -y.toInt := by omega
-    simp only [this]; clear this
-
-    have : (-x.toInt) / (-y.toInt) = (-x.toInt).tdiv (-y.toInt) := by
-      rw [Int.tdiv_eq_ediv]; omega
-    rw [this]
-    simp only [Int.tdiv_neg, Int.neg_tdiv, neg_neg]
-
 uscalar theorem «%S».div_bv_spec (x : «%S») {y : «%S»} (hnz : ↑y ≠ (0 : Nat)) :
-  x /? y ⦃ z => (↑z : Nat) = ↑x / ↑y ∧ z.toBitVec = x.toBitVec / y.toBitVec ⦄ :=
-  exists_imp_spec (UScalar.div_toBitVec_spec x hnz)
+  x /? y ⦃ z => (↑z : Nat) = ↑x / ↑y ∧ z.toBitVec = x.toBitVec / y.toBitVec ⦄ := by
+  change @spec _ (x.div y) _
+  apply exists_imp_spec
+  have hzero' : y.toBitVec ≠ BitVec.ofNat _ 0 := by
+    intro h
+    zify at h
+    simp_all
+  simp [hzero', div]; rfl
 
 iscalar theorem «%S».div_bv_spec {x y : «%S»} (hnz : ↑y ≠ (0 : Int))
   (hNoOverflow : ¬ (x.toInt = «%S».min ∧ y.toInt = -1)) :
