backends/lean/Aeneas/Std/Scalar/Ops/Rem.lean
@@ -11,12 +11,6 @@ open Result Error Arith ScalarElab WP
 /-!
 # Remainder: Definitions
 -/
-def UScalar.rem {ty : UScalarTy} (x y : UScalar ty) : Result (UScalar ty) :=
-  if y.toNat != 0 then ok ⟨ BitVec.umod x.toBitVec y.toBitVec ⟩ else fail divisionByZero
-
-def IScalar.rem {ty : IScalarTy} (x y : IScalar ty) : Result (IScalar ty) :=
-  if y.toInt != 0 then ok ⟨ BitVec.srem x.toBitVec y.toBitVec ⟩
-  else fail divisionByZero
 
 uscalar def «%S».rem (x y : «%S») : Result «%S» :=
   if y.toNat != 0 then ok ⟨ BitVec.umod x.toBitVec y.toBitVec ⟩ else fail divisionByZero
@@ -25,22 +19,10 @@ iscalar def «%S».rem (x y : «%S») : Result «%S» :=
   if y.toInt != 0 then ok ⟨ BitVec.srem x.toBitVec y.toBitVec ⟩
   else fail divisionByZero
 
-def UScalar.try_rem {ty : UScalarTy} (x y : UScalar ty) : Option (UScalar ty) :=
-  Option.ofResult (rem x y)
-
-def IScalar.try_rem {ty : IScalarTy} (x y : IScalar ty) : Option (IScalar ty) :=
-  Option.ofResult (rem x y)
-
 class ResultMod (α : Type u) where
   mod : α → α → Result α
 
 infixl:70 " %? " => ResultMod.mod
-
-instance {ty} : ResultMod (UScalar ty) where
-  mod x y := UScalar.rem x y
-
-instance {ty} : ResultMod (IScalar ty) where
-  mod x y := IScalar.rem x y
 
 scalar instance : ResultMod «%S» where
   mod x y := «%S».rem x y
@@ -89,20 +71,6 @@ end Tests
 /-!
 Theorems with a specification which uses integers and bit-vectors
 -/
-
-theorem UScalar.rem_toBitVec_spec {ty} (x : UScalar ty) {y : UScalar ty} (hzero : y.toNat ≠ 0) :
-  x %? y ⦃ z => (↑z : Nat) = ↑x % ↑y ∧ z.toBitVec = x.toBitVec % y.toBitVec ⦄ := by
-  conv => arg 1; simp [ResultMod.mod]
-  simp [hzero, rem]
-  simp only [toNat]
-  simp
-
-theorem IScalar.rem_toBitVec_spec {ty} (x : IScalar ty) {y : IScalar ty} (hzero : y.toInt ≠ 0) :
-  x %? y ⦃ z => (↑z : Int) = Int.tmod ↑x ↑y ∧ z.toBitVec = BitVec.srem x.toBitVec y.toBitVec ⦄ := by
-  conv => arg 1; simp [ResultMod.mod]
-  simp only [spec_ok, rem, bne_iff_ne, ne_eq, hzero, not_false_eq_true, ↓reduceIte]
-  simp only [toInt]
-  simp only [BitVec.toInt_srem, toBitVec_toInt_eq, and_true]
 
 uscalar theorem «%S».rem_bv_spec (x : «%S») {y : «%S»} (hnz : y.toNat ≠ 0) :
   x %? y ⦃ z => (↑z : Nat) = ↑x % ↑y ∧ z.toBitVec = x.toBitVec % y.toBitVec ⦄ := by
